Manual/Meta.lean
@@ -24,7 +24,9 @@ import Manual.Meta.Example
 import Manual.Meta.Figure
 import Manual.Meta.Lean
 import Manual.Meta.Marginalia
+import Manual.Meta.ParserAlias
 import Manual.Meta.Syntax
+import Manual.Meta.Table
 import Manual.Meta.Tactics
 
 open Lean Elab
