Manual/Meta/ParserAlias.lean
@@ -1,0 +1,125 @@
+/-
+Copyright (c) 2024 Lean FRO LLC. All rights reserved.
+Released under Apache 2.0 license as described in the file LICENSE.
+Author: David Thrane Christiansen
+-/
+
+import Lean.Elab.Term
+import Lean.Elab.Tactic
+
+import Verso.Code.Highlighted
+import Verso.Doc.ArgParse
+import Verso.Doc.Suggestion
+import SubVerso.Highlighting.Code
+import VersoManual
+
+import Manual.Meta.Basic
+import Manual.Meta.PPrint
+import Manual.Meta.Lean
+import Manual.Meta.Lean.Scopes
+
+namespace Manual
+
+open Lean Elab Term Tactic
+open Verso ArgParse Doc Elab Genre.Manual Html Code Highlighted.WebAssets
+open Manual.Meta.Lean.Scopes
+open SubVerso.Highlighting
+
+def parserAliasDomain := `Manual.parserAlias
+
+def Block.parserAlias (name : Name) (declName : Name) («show» : Option String) (stackSz? : Option Nat) (autoGroupArgs : Bool) (docs? : Option String) (argCount : Nat) : Block where
+  name := `Manual.Block.parserAlias
+  data := ToJson.toJson (name, declName, «show», stackSz?, autoGroupArgs, docs?, argCount)
+
+structure ParserAliasOptions where
+  name : Name
+  «show» : Option String
+
+def ParserAliasOptions.parse [Monad m] [MonadError m] : ArgParse m ParserAliasOptions :=
+  ParserAliasOptions.mk <$> .positional `name .name <*> .named `show .string true
+
+
+
+@[directive_expander parserAlias]
+def parserAlias : DirectiveExpander
+  | args, more => do
+    let opts ← ParserAliasOptions.parse.run args
+    let {declName, stackSz?, autoGroupArgs} ← Parser.getParserAliasInfo opts.name
+    let docs? ← findDocString? (← getEnv) declName
+
+    let some mdAst := MD4Lean.parse (docs?.getD "")
+      | throwError "Failed to parse docstring as Markdown"
+    let contents ← mdAst.blocks.mapM (Markdown.blockFromMarkdown · Markdown.strongEmphHeaders)
+    let userContents ← more.mapM elabBlock
+
+    let argCount :=
+      match (← Lean.Parser.getAlias Lean.Parser.parserAliasesRef opts.name) with
+      | some (.unary ..) => 1
+      | some (.binary ..) => 2
+      | _ => 0
+
+    pure #[← ``(Verso.Doc.Block.other (Block.parserAlias $(quote opts.name) $(quote declName) $(quote opts.show) $(quote stackSz?) $(quote autoGroupArgs) $(quote docs?) $(quote argCount)) #[$(contents ++ userContents),*])]
+
+
+open Verso.Genre.Manual.Markdown in
+open Lean Elab Term Parser Tactic Doc in
+@[block_extension Block.parserAlias]
+def parserAlias.descr : BlockDescr where
+  init st := st
+    |>.setDomainTitle parserAliasDomain "Parser Alias Documentation"
+    |>.setDomainDescription parserAliasDomain "Detailed descriptions of parser aliases"
+
+  traverse id info _ := do
+    let .ok (name, _declName, «show», _stackSz?, _autoGroupArgs, _docs?, _) := FromJson.fromJson? (α := Name × Name × Option String × Option Nat × Bool × Option String × Nat) info
+      | do logError "Failed to deserialize docstring data while traversing a parser alias"; pure none
+    let path ← (·.path) <$> read
+    let _ ← Verso.Genre.Manual.externalTag id path <| show.getD name.toString
+    Index.addEntry id {term := Doc.Inline.code <| show.getD name.toString}
+
+    modify fun st => st.saveDomainObject parserAliasDomain name.toString id
+
+    pure none
+  toHtml := some <| fun _goI goB id info contents =>
+    open Verso.Doc.Html in
+    open Verso.Output Html in do
+      let .ok (name, declName, «show», stackSz?, autoGroupArgs, docs?, argCount) := FromJson.fromJson? (α := Name × Name × Option String × Option Nat × Bool × Option String × Nat) info
+        | do Verso.Doc.Html.HtmlT.logError "Failed to deserialize parser alias data while generating HTML for a parser alias docstring"; pure .empty
+      let x : Highlighted := .token ⟨.keyword declName none docs?, show.getD name.toString⟩
+      let args : Highlighted :=
+        match argCount with
+        | 1 => .seq <|
+          #[.token ⟨.unknown, "("⟩, .token ⟨.unknown, "p"⟩, .token ⟨.unknown, ")"⟩]
+        | 2 => .seq <|
+          #[.token ⟨.unknown, "("⟩, .token ⟨.unknown, "p1"⟩, .token ⟨.unknown, ", "⟩, .token ⟨.unknown, "p2"⟩, .token ⟨.unknown, ")"⟩]
+        | _ => .empty
+
+      let xref ← HtmlT.state
+      let idAttr := xref.htmlId id
+
+      let arity :=
+        match stackSz? with
+        | some n => s!"Arity: {n}"
+        | none => "Arity is sum of arguments' arities"
+      let grp :=
+        if autoGroupArgs then
+          some {{"Automatically wraps arguments in a " <code>"null"</code> " node unless there's exactly one"}}
+        else none
+      let meta :=
+        match grp with
+        | none => {{<p>{{arity}}</p>}}
+        | some g => {{<ul><li>{{arity}}</li><li>{{g}}</li></ul>}}
+
+      return {{
+        <div class="namedocs" {{idAttr}}>
+          {{permalink id xref false}}
+          <span class="label">"parser alias"</span>
+          <pre class="signature hl lean block">{{← (Highlighted.seq #[x, args]).toHtml}}</pre>
+          <div class="text">
+            {{meta}}
+            {{← contents.mapM goB}}
+          </div>
+        </div>
+      }}
+  toTeX := none
+  extraCss := [highlightingStyle, docstringStyle]
+  extraJs := [highlightingJs]
