Manual/Meta/Table.lean
@@ -1,0 +1,132 @@
+/-
+Copyright (c) 2024 Lean FRO LLC. All rights reserved.
+Released under Apache 2.0 license as described in the file LICENSE.
+Author: David Thrane Christiansen
+-/
+
+import VersoManual
+import Lean.Elab.InfoTree.Types
+
+import Manual.Meta.Figure
+
+open Verso Doc Elab
+open Verso.Genre Manual
+open Verso.ArgParse
+
+open Lean Elab
+
+set_option pp.rawOnError true
+
+namespace Manual
+
+def Block.table (columns : Nat) (header : Bool) (name : Option String) : Block where
+  name := `Manual.table
+  data := ToJson.toJson (columns, header, name, (none : Option Tag))
+
+structure TableConfig where
+  /-- Name for refs -/
+  name : Option String := none
+  header : Bool := false
+
+
+def TableConfig.parse [Monad m] [MonadInfoTree m] [MonadLiftT CoreM m] [MonadEnv m] [MonadError m] [MonadFileMap m] : ArgParse m TableConfig :=
+  TableConfig.mk <$> .named `tag .string true <*> ((·.getD false) <$> .named `header .bool true)
+
+@[directive_expander table]
+def table : DirectiveExpander
+  | args, contents => do
+    let cfg ← TableConfig.parse.run args
+    -- The table should be a list of lists. Extract them!
+    let #[contentStx@`<low|(Verso.Syntax.ul ~(.node _ `null items) )>] := contents
+      | throwError "Expected a single unordered list"
+    let preRows ← items.mapM getLi
+    let rows ← preRows.mapM fun blks => do
+      let #[`<low|(Verso.Syntax.ul ~(.node _ `null cellItems) )>] := blks.filter (·.isOfKind ``Verso.Syntax.ul)
+        | throwError "Each row should have exactly one list in it"
+      cellItems.mapM getLi
+    if h : rows.size = 0 then
+      throwErrorAt contentStx "Expected at least one row"
+    else
+      let columns := rows[0].size
+      if columns = 0 then
+        throwErrorAt contentStx "Expected at least one column"
+      if rows.any (·.size != columns) then
+        throwErrorAt contentStx s!"Expected all rows to have same number of columns, but got {rows.map (·.size)}"
+
+      let flattened := rows.flatten
+      let blocks : Array (Syntax.TSepArray `term ",") ← flattened.mapM (·.mapM elabBlock)
+      -- Figures are represented using the first block to hold the caption. Storing it in the JSON
+      -- entails repeated (de)serialization.
+      pure #[← ``(Block.other (Block.table $(quote columns) $(quote cfg.header) $(quote cfg.name)) #[Block.ul #[$[Verso.Doc.ListItem.mk 0 #[$blocks,*]],*]])]
+
+where
+  getLi
+    | `<low|(Verso.Syntax.li ~_ ~(.node _ `null content) )> => pure content
+    | other => throwErrorAt other "Expected list item"
+
+
+@[block_extension table]
+def table.descr : BlockDescr where
+  traverse id data contents := do
+    match FromJson.fromJson? data (α := Nat × Bool × Option String × Option Tag) with
+    | .error e => logError s!"Error deserializing table data: {e}"; pure none
+    | .ok (_, _, none, _) => pure none
+    | .ok (c, hdr, some x, none) =>
+      let path ← (·.path) <$> read
+      let tag ← Verso.Genre.Manual.externalTag id path x
+      pure <| some <| Block.other {Block.table c hdr none with id := some id, data := toJson (c, some x, some tag)} contents
+    | .ok (_, _, some _, some _) => pure none
+  toTeX := none
+  toHtml :=
+    open Verso.Doc.Html in
+    open Verso.Output.Html in
+    some <| fun goI goB id data blocks => do
+      match FromJson.fromJson? data (α := Nat × Bool × Option String × Option Tag) with
+      | .error e =>
+        HtmlT.logError s!"Error deserializing table data: {e}"
+        return .empty
+      | .ok (columns, header, _, _) =>
+      if let #[.ul items] := blocks then
+        let xref ← HtmlT.state
+        let attrs := xref.htmlId id
+        let mut items := items
+        let mut rows := #[]
+        while items.size > 0 do
+          rows := rows.push (items.take columns |>.map (·.contents))
+          items := items.extract columns items.size
+
+        return {{
+          <table class="tabular" {{attrs}}>
+            {{← rows.mapIdxM fun i r => do
+              let cols ← Output.Html.seq <$> r.mapM fun c => do
+                let cell : Output.Html ← c.mapM goB
+                if header && i == 0 then
+                  pure {{<th>{{cell}}</th>}}
+                else
+                  pure {{<td>{{cell}}</td>}}
+              pure {{<tr>{{cols}}</tr>}}
+            }}
+          </table>
+        }}
+
+      else
+        HtmlT.logError "Malformed table"
+        return .empty
+  extraCss := [
+r##"
+table.tabular {
+  margin: auto;
+  border-spacing: 1rem;
+}
+table.tabular td, table.tabular th {
+  text-align: left;
+  vertical-align: top;
+}
+table.tabular td > p:first-child, table.tabular th > p:first-child {
+  margin-top: 0;
+}
+table.tabular td > p:last-child, table.tabular th > p:first-child {
+  margin-bottom: 0;
+}
+"##
+  ]
