Manual/Papers.lean
@@ -1,0 +1,50 @@
+/-
+Copyright (c) 2024 Lean FRO LLC. All rights reserved.
+Released under Apache 2.0 license as described in the file LICENSE.
+Author: David Thrane Christiansen
+-/
+
+import Manual.Meta.Bibliography
+
+open Manual
+
+def beyondNotations : InProceedings where
+  title := .concat (inlines!"Beyond notations: Hygienic macro expansion for theorem proving languages")
+  authors := #[.concat (inlines!"Sebastian Ullrich"), .concat (inlines!"Leonardo de Moura")]
+  year := 2020
+  booktitle := .concat (inlines!"Proceedings of the International Joint Conference on Automated Reasoning")
+
+
+def carneiro19 : Thesis where
+  title := .concat (inlines!"The Type Theory of Lean")
+  author := .concat (inlines!"Mario Carneiro")
+  year := 2019
+  university := .concat (inlines!"Carnegie Mellon University")
+  url := some "https://github.com/digama0/lean-type-theory/releases/download/v1.0/main.pdf"
+  degree := .concat (inlines!"Masters thesis")
+
+def castPaper : ArXiv where
+  title := .concat (inlines!"Simplifying Casts and Coercions")
+  authors := #[.concat (inlines!"Robert Y. Lewis"), .concat (inlines!"Paul-Nicolas Madelaine")]
+  year := 2020
+  id := "2001.10594"
+
+def pratt73 : InProceedings where
+  title := .concat (inlines!"Top down operator precedence")
+  authors := #[.concat (inlines!"Vaughan Pratt")]
+  year := 1973
+  booktitle := .concat (inlines!"Proceedings of the 1st Annual ACM SIGACT-SIGPLAN Symposium on Principles of Programming Languages")
+
+def tabledRes : ArXiv where
+  title := .concat (inlines!"Tabled typeclass resolution")
+  authors := #[.concat (inlines!"Daniel Selsam"), .concat (inlines!"Sebastian Ullrich"), .concat (inlines!"Leonardo de Moura")]
+  year := 2020
+  id := "2001.04301"
+
+def ullrich23 : Thesis where
+  title := .concat (inlines!"An Extensible Theorem Proving Frontend")
+  author := .concat (inlines!"Sebastian Ullrich")
+  year := 2023
+  university := .concat (inlines!"Karlsruhe Institute of Technology")
+  url := some "https://www.lean-lang.org/papers/thesis-sebastian.pdf"
+  degree := .concat (inlines!"Dr. Ing. dissertation")
